%! TEX root = ./main.tex
\documentclass[12pt]{article}

%--------Packages-------------
\usepackage{kyrem1sty}
%----------------------------


%--------Bibliography---------
%\usepackage[backend=biber]{biblatex}
%\addbibresource{INSERT .BIB PATH}
%----------------------------


%--------Subfiles Setup-------
\usepackage{subfiles}
%----------------------------


%--------Page Setup-----------
%\usepackage{geometry}\geometry{margin=1in}
\pagestyle{empty}%

\setlength{\hoffset}{-1.54cm}
\setlength{\voffset}{-1.54cm}

\setlength{\topmargin}{0pt}
\setlength{\headsep}{0pt}
\setlength{\headheight}{0pt}

\setlength{\oddsidemargin}{0pt}

\setlength{\textwidth}{195mm}
\setlength{\textheight}{250mm}
%----------------------------


%--------Metadata------------
\title{Algebraic Actions Notes}
\author{James Harbour}
%----------------------------


%--------Content-------------
\begin{document}
\maketitle

    We then note that
    \begin{equation}\begin{split}
        \sum_{r=1}^{\delta n} \frac{1}{r} {(s+1)r-2 \choose r-1} \cdot \lr{\frac{s^s}{(s+1)^{(s+1)}}}^{r} = \\
        \sum_{r=1}^{\delta n} \frac{1}{(s+1)r-1} {(s+1)r-1 \choose r} \cdot \lr{\frac{s^s}{(s+1)^{(s+1)}}}^{r} = \\
        1 + \sum_{r=0}^{\delta n} \frac{1}{(s+1)r-1} {(s+1)r-1 \choose r} \cdot \lr{\frac{s^s}{(s+1)^{(s+1)}}}^{r} = \\
        1 - \sum_{r=0}^{\delta n} \frac{-1}{(s+1)r-1} {(s+1)r-1 \choose r} \cdot \lr{\frac{s^s}{(s+1)^{(s+1)}}}^{r}
    \end{split}\end{equation}
    
    Let us note that if we apply Lemma \ref{lem:polya_szego} with $a = -1$, $b = s+1$, and $k = r$, we have
    \begin{equation}\begin{split}
        \sum_{r=0}^{\infty} \frac{-1}{(s+1)r-1} {(s+1)r - 1 \choose r} z^r = \frac{1}{x}
    \end{split}\end{equation}

    Provided that we meet the conditions
    \begin{align}
        z = \frac{x - 1}{x^{(s+1)}} && |z| < \frac{s^s}{(s+1)^{(s+1)}}
    \end{align}
    
       We then note that for $\frac{s}{s+1} < \gamma < 1$, if we set $x = \gamma \frac{s+1}{s}$, then
    \begin{equation}\begin{split}
        |z| = \abs{\frac{\gamma \frac{s+1}{s} - 1}{(\gamma \frac{s+1}{s})^{(s+1)}}} = \frac{1}{\gamma^s} \cdot \frac{s^s}{(s+1)^{(s+1)}} \cdot \abs{\lr{s\lr{1 - \frac{1}{\gamma}} + 1}} < \frac{s^s}{(s+1)^{(s+1)}}
    \end{split}\end{equation}1
        Therefore, if $x = \gamma \frac{s+1}{s}$ and $z = \frac{x - 1}{x^{(s+1)}}$, then we have
    \begin{equation}\begin{split}
        \sum_{r=0}^{\infty} \frac{-1}{(s+1)r-1} {(s+1)r - 1 \choose r} z^r = \frac{1}{\gamma } \frac{s}{s+1}
    \end{split}\end{equation}

    \newpage

Consider the function $ F:(0,+\infty)\to \R $ given by
\[
    F(\gamma) = \frac{\gamma \frac{s+1}{s} - 1}{(\gamma \frac{s+1}{s})^{(s+1)}} = \frac{1}{\gamma^s} \cdot \frac{s^s}{(s+1)^{(s+1)}} \cdot \lr{s\lr{1 - \frac{1}{\gamma}} + 1}
\]
This function is nonnegative and monotone increasing for $\gamma \in (\frac{s}{s+1},1) $. Moreover, in this range we have 
\begin{align*}
    \sum_{r=0}^{\infty} \frac{-1}{(s+1)r-1} {(s+1)r - 1 \choose r} F(\gamma)^r = \frac{1}{\gamma} \frac{s}{s+1} 
\end{align*}
whence
\[
    1-\frac{1}{\gamma}\frac{s}{s+1} = \sum_{r=1}^{\infty} \frac{1}{(s+1)r-1} {(s+1)r - 1 \choose r} F( \gamma)^{r}
\]

Let $ (\eps_{k})_{k} $ be a sequence increasing to $ 1 $ with $ \eps_{k}> \frac{s}{s+1} $ for all $ k\in \N $, and define 
\[
    a_{r,k} = \frac{1}{(s+1)r -1} \binom{(s+1)r -1}{r} F(\eps_{k})^{r}.
\]
As $ F $ is monotone increasing in the range of the $ \eps_{k} $s, we have $ a_{r,k}\leq a_{r,k+1} $ for all $ r,k\in \N $. By the monotone convergence theorem,
\begin{align*}
    \sum_{r=1}^{\infty} \frac{1}{(s+1)r-1}&\binom{(s+1)r-1}{r} \lr{\frac{s^{s}}{(s+1)^{s+1}}}^{r} \\
    &=  \sum_{r=1}^{\infty} \sup_{k} a_{r,k}  
    = \sup_{k}\sum_{r=1}^{\infty}  a_{r,k} = \sup_{k} 1- \frac{1}{\eps_{k}} \frac{s}{s+1} = 1-\frac{s}{s+1}
\end{align*}
or equivalently
\begin{equation*}
    \sum_{r=0}^{\infty} \frac{-1}{(s+1)r-1} {(s+1)r - 1 \choose r} \cdot \left( \frac{s^s}{(s+1)^{(s+1)}} \right)^r  = \frac{s}{s+1}.
\end{equation*}



  Equivalently (plugging in $z$), we have
    \begin{equation}\begin{split}
        \sum_{r=0}^{\infty} \frac{-1}{(s+1)r-1} {(s+1)r - 1 \choose r} \cdot \left( \frac{s^s}{(s+1)^{(s+1)}} \right)^r \cdot \left( \gamma^{s} \cdot (1 - s (1 - \gamma)) \right)^r = \gamma \frac{s}{s+1}
    \end{split}\end{equation}


    
    \textbf{TODO: insert justification for why this converges at the radius}


    
    We then have
    \begin{equation}\begin{split}
        1 - \sum_{r=0}^{\delta n} \frac{-1}{(s+1)r-1} {(s+1)r-1 \choose r} \cdot \lr{\frac{s^s}{(s+1)^{(s+1)}}}^{r} \sim \frac{1}{s+1}
    \end{split}\end{equation}


\end{document}
